6

**B–5** **First solution:** Put $Q = x_1^2 + \dots + x_n^2$. Since $Q$ is homogeneous, $P$ is divisible by $Q$ if and only if each of the homogeneous components of $P$ is divisible by $Q$. It is thus sufficient to solve the problem in case $P$ itself is homogeneous, say of degree $d$.

Suppose that we have a factorization $P = Q^m R$ for some $m > 0$, where $R$ is homogeneous of degree $d$ and not divisible by $Q$; note that the homogeneity implies that

$$ \sum_{i=1}^n x_i \frac{\partial R}{\partial x_i} = dR. $$

Write $\nabla^2$ as shorthand for $\frac{\partial^2}{\partial x_1^2} + \dots + \frac{\partial^2}{\partial x_n^2}$; then

$$
\begin{aligned}
0 &= \nabla^2 P \\
  &= 2mn Q^{m-1} R + Q^m \nabla^2 R + 2 \sum_{i=1}^n 2m x_i Q^{m-1} \frac{\partial R}{\partial x_i} \\
  &= Q^m \nabla^2 R + (2mn + 4md) Q^{m-1} R.
\end{aligned}
$$

Since $m > 0$, this forces $R$ to be divisible by $Q$, contradiction.

**Second solution:** (by Noam Elkies) Retain notation as in the first solution. Let $P_d$ be the set of homogeneous polynomials of degree $d$, and let $H_d$ be the subset of $P_d$ of polynomials killed by $\nabla^2$, which has dimension $\ge \dim(P_d) - \dim(P_{d-2})$; the given problem amounts to showing that this inequality is actually an equality.

Consider the operator $Q\nabla^2$ (i.e., apply $\nabla^2$ then multiply by $Q$) on $P_d$; its zero eigenspace is precisely $H_d$. By the calculation from the first solution, if $R \in P_d$, then

$$ \nabla^2(QR) - Q\nabla^2 R = (2n + 4d)R. $$

Consequently, $Q^j H_{d-2j}$ is contained in the eigenspace of $Q\nabla^2$ on $P_d$ of eigenvalue

$$ (2n + 4(d-2j)) + \dots + (2n + 4(d-2)). $$

In particular, the $Q^j H_{d-2j}$ lie in distinct eigenspaces, so are linearly independent within $P_d$. But by dimension counting, their total dimension is at least that of $P_d$. Hence they exhaust $P_d$, and the zero eigenspace cannot have dimension greater than $\dim(P_d) - \dim(P_{d-2})$, as desired.

**Third solution:** (by Richard Stanley) Write $x = (x_1, \dots, x_n)$ and $\nabla = (\frac{\partial}{\partial x_1}, \dots, \frac{\partial}{\partial x_n})$. Suppose that $P(x) = Q(x)(x_1^2 + \dots + x_n^2)$. Then

$$ P(\nabla)P(x) = Q(\nabla)(\nabla^2)P(x) = 0. $$

On the other hand, if $P(x) = \sum_\alpha c_\alpha x^\alpha$ (where $\alpha = (\alpha_1, \dots, \alpha_n)$ and $x^\alpha = x_1^{\alpha_1} \dots x_n^{\alpha_n}$), then the constant term of $P(\nabla)P(x)$ is seen to be $\sum_\alpha c_\alpha^2$. Hence $c_\alpha = 0$ for all $\alpha$.

**Remarks:** The first two solutions apply directly over any field of characteristic zero. (The result fails in characteristic $p > 0$ because we may take $P = (x_1^2 + \dots + x_n^2)^p = x_1^{2p} + \dots + x_n^{2p}$.) The third solution can be extended to complex coefficients by replacing $P(\nabla)$ by its complex conjugate, and again the result may be deduced for any field of characteristic zero. Stanley also suggests Section 5 of the arXiv e-print math.CO/0502363 for some algebraic background for this problem.

**B–6** **First solution:** Let $I$ be the identity matrix, and let $J_x$ be the matrix with $x$'s on the diagonal and $1$'s elsewhere. Note that $J_x - (x-1)I$, being the all $1$'s matrix, has rank 1 and trace $n$, so has $n-1$ eigenvalues equal to $0$ and one equal to $n$. Hence $J_x$ has $n-1$ eigenvalues equal to $x-1$ and one equal to $x+n-1$, implying

$$ \det J_x = (x+n-1)(x-1)^{n-1}. $$

On the other hand, we may expand the determinant as a sum indexed by permutations, in which case we get

$$ \det J_x = \sum_{\pi \in S_n} \text{sgn}(\pi) x^{\nu(\pi)}. $$

Integrating both sides from 0 to 1 (and substituting $y = 1-x$) yields

$$
\begin{aligned}
\sum_{\pi \in S_n} \frac{\text{sgn}(\pi)}{\nu(\pi)+1} &= \int_0^1 (x+n-1)(x-1)^{n-1} \, dx \\
&= \int_0^1 (-1)^{n+1} (n-y) y^{n-1} \, dy \\
&= (-1)^{n+1} \frac{n}{n+1},
\end{aligned}
$$

as desired.

**Second solution:** We start by recalling a form of the principle of inclusion-exclusion: if $f$ is a function on the power set of $\{1, \dots, n\}$, then

$$ f(S) = \sum_{T \supseteq S} (-1)^{|T|-|S|} \sum_{U \supseteq T} f(U). $$

In this case we take $f(S)$ to be the sum of $\sigma(\pi)$ over all permutations $\pi$ whose fixed points are exactly $S$. Then $\sum_{U \supseteq T} f(U) = 1$ if $|T| \ge n-1$ and $0$ otherwise (since a permutation group on 2 or more symbols has as many even and odd permutations), so

$$ f(S) = (-1)^{n-|S|} (1 - n + |S|). $$

The desired sum can thus be written, by grouping over fixed point sets, as

$$
\begin{aligned}
\sum_{i=0}^n \binom{n}{i} (-1)^{n-i} \frac{1-n+i}{i+1} \\
&= \sum_{i=0}^n (-1)^{n-i} \binom{n}{i} - \sum_{i=0}^n (-1)^{n-i} \frac{n}{i+1} \binom{n}{i} \\
&= 0 - \sum_{i=0}^n (-1)^{n-i} \frac{n}{n+1} \binom{n+1}{i+1} \\
&= (-1)^{n+1} \frac{n}{n+1}.
\end{aligned}
$$